---
title: $\dim M$ ä¸ $\dim (T,M)$
author: Chencheng Zhang
layout: post
category: proof
---
## è¯æ˜

{% lem %}

($ğ’¯$, $ğ’´$ ä¸æŠ•å°„ç»´æ•°). å¯¹ $M âˆˆ ğ’¯$.

1. è‹¥ $p.\dim M â‰  1$, åˆ™ $p.\dim M = p.\dim (T,M)$.
2. è‹¥ $p.\dim M = 1$, åˆ™ $p.\dim (T,M)$ ä¸º $0$ æˆ– $1$.

{% endlem %}

{% pf %}
ä½¿ç”¨æ•°å­¦å½’çº³æ³•.

1. å‡å®š $p.\dim M = 0$. æ­¤æ—¶ $M$ æŠ•å°„. ç”± $M âˆˆ \mathrm{Gen}(T)$ çŸ¥ $M âˆˆ ğšğğ(T)$. å› æ­¤ $p.\dim (T,M) = 0$.
2. å‡å®š $p.\dim M = 1$. å–å³é€¼è¿‘çš„ ses $Î¸ : 0 â†’ K â†’ T^n â†’ M â†’ 0$ ä½¿å¾— $K âˆˆ ğ’¯$. æ­¤æ—¶ $(T, Î¸)$-æ­£åˆ, åªéœ€è¯æ˜ $K âˆˆ ğšğğ(T)$. ç­‰ä»·åœ°, $\mathrm{Ext}^1(K, ğ’¯) = 0$, è€ƒè™‘ä»¥ä¸‹ ses å³å¯:

    $$
    0 â†’ \underset{\text{ses}}{\underbrace{(M, ğ’¯) â†’ (T^n, ğ’¯) â†’ (K, ğ’¯)}} â†’ {}^1(M, ğ’¯) â†’ {}^1 (T^n, ğ’¯) = 0.
    $$

3. (å½’çº³). å‡å®š $p.\dim M = n+1 â‰¥ 2$, åªéœ€è¯æ˜ $p.\dim (T,K) â‰¤ n$. ç”±å½’çº³å‡è®¾, åªéœ€è¯æ˜ $p.\dim K â‰¤ n$. ç”±

   $$
   0 â†’ \underset{p.\dim = ?}{\underbrace{K}} â†’ \underset{p.\dim â‰¤ 1}{\underbrace{T^n}} â†’ \underset{p.\dim = n + 1}{\underbrace{M}} â†’ 0,
   $$

   å› æ­¤ $p.\dim K = p.\dim M - 1 = n + 1$.

å…³äºå–ç­‰æ¡ä»¶çš„è®¨è®ºå¦‚ä¸‹.

1. $p. \dim M = 0$ æ—¶ $p. \dim (T, M) = 0$.
2. $p.\dim M = 1$ æ—¶ $p.\dim (T,M) âˆˆ \{0,1\}$. ä¾‹å¦‚å– $M = T âˆ‰ ğ©ğ«ğ¨ğ£$, åˆ™ $p.\dim T = 1$ ä½† $p.\dim (T, M) = 0$.
3. $p.\dim M = n â‰¥ 2$ æ—¶ $p.\dim (T, M) â‰¥ 2$: è€ƒè™‘å‡½å­çš„æ­£åˆåˆ—:

    $$
    \mathrm{Ext}{}^1 (M, -)â†’\mathrm{Ext}{}^1 (T^n, -)â†’\mathrm{Ext}{}^1 (K, -)â†’ \mathrm{Ext}{}^2(M, -) â†’ 0 â†’ \cdots.
    $$

    ä»¥åŠ

    $$
    \cdots â†’ 0 â†’ \mathrm{Ext}{}^{k} (K, -) â‰ƒ \mathrm{Ext}{}^{k+1} (M, -) â†’ 0 â†’ \cdots\quad (k â‰¥ 2).
    $$

    æ­¤æ—¶ $\mathrm{Ext}{}^{1,\ldots, n-1} (K, -) â‰  0$, ä½† $\mathrm{Ext}{}^n(K, -) =0$.

{% endpf %}
