---
title: é—ä¼ èŒƒç•´çš„ $\mathrm{Hom}_{Dğ’œ}(-,-)$.
author: Chencheng Zhang
layout: post
category: proof
---
## è¯æ˜

{% thm %}
é—ä¼ èŒƒç•´ä¸­, $X^âˆ™$ ä¸ $H^âˆ™(X)$ (åŒè°ƒç¾¤æ„æˆçš„è½´å¤å½¢) å¯¼å‡ºç­‰ä»·.
{% endthm %}

{% pf %}
ç»™å®šä¸Šé“¾å¤å½¢ $(X^âˆ™, d^âˆ™)$. è€ƒè™‘ $X^n$ é™„è¿‘çš„äº¤æ¢å›¾

$$
\begin{bmatrix}
r_{1} : & \cdots  & \rightarrow  & X^{n-2} & \rightarrow  & X^{n-1} & \xrightarrow{d^{n-1}} & X^{n} & \xrightarrow{d^{n}} & X^{n+1} & \rightarrow  & \cdots \\
\uparrow  &  &  & \uparrow  &  & \parallel  & âŠ   & \uparrow  &  & \uparrow  &  & \\
r_{2} : & \cdots  & \rightarrow  & 0 & \rightarrow  & X^{n-1} & \hookrightarrow  & E & \rightarrow  & 0 & \rightarrow  & \cdots \\
\Downarrow  &  &  & \Downarrow  &  & \Downarrow  &  & \Downarrow  &  & \Downarrow  &  & \\
r_{3} : & \cdots  & \rightarrow  & 0 & \rightarrow  & 0 & \rightarrow  & H^{n}( X) & \rightarrow  & 0 & \rightarrow  & \cdots 
\end{bmatrix}.
$$

æ­¤å¤„, äº¤æ¢æ–¹å— $âŠ $ å†…éƒ¨å¦‚ä¸‹ ($â–¦$ æ˜¯æ¨å‡ºæ‹‰å›):

$$
âŠ  = \begin{bmatrix}
X^{n-1} & = & X^{n-1} & \xrightarrow{d^{n-1}} & X^{n}\\
\parallel  &  & â†¡  &  & \uparrow \\
\parallel  &  & \operatorname{im} d^{n-1} & â†ª  & \ker d^{n}\\
\parallel  &  & â†Ÿ  & â–¦ & â†Ÿ \\
X^{n-1} & = & X^{n-1} & \rightarrow  & E
\end{bmatrix}.
$$

ç‰¹åˆ«åœ°, $r_2 â‡’ r_3$ æ˜¯æ‹ŸåŒæ„, $r_2 â†’ r_1$ ä»…æŠ•å½± $X^n$ å¤„åŒè°ƒç¾¤. å°† $r_2$ å–éæ‰€æœ‰ $X^k â†ª E'$, å¾—æ‹ŸåŒæ„

$$
X^âˆ™ â‡ âˆ‘\limits_k [X^k â†ª E'] â‡’ H^âˆ™ (X).
$$

{% endpf %}
