---
title: CT5
author: ZCC
layout: post
category: note
---

* toc
{: toc}

## Lecture 5

## CT Generated by Pure Injectives

### Technique: Tor-torsion Theory

A tor-torsion theory induces a cotorsion theory with good proeprty.

{% def %}
Say $(\mathcal{A}, \mathcal{B})$ consists of a tor-torsion theory, provided

$$\begin{equation}
\mathcal{A}^⊺ := \ker \mathrm{Tor}(\mathcal{A}, -) = \mathcal{B}; \quad {}^⊺\mathcal{B} := \ker \mathrm{Tor}(-, \mathcal{B}) = \mathcal{A}.
\end{equation}$$

{% enddef %}

{% pro %}
Show that both $\mathcal{A}$ and $\mathcal{B}$ are closed under summands, extensions, and filtered colimits.

- In general, the left derives of the left adjoint commutes with filtered colimits.

{% endpro %}

The following lemma ***embeds*** the tor-torsion theory into general cotorsion theory.

{% lem %}
For any $X ∈ 𝐌𝐨𝐝 _R$ and $Y ∈ 𝐌𝐨𝐝 _{R^{\mathrm{op}}}$, $\mathrm{Ext}^1(X,Y^+) =0$ **iff** $\mathrm{Tor}_1(X,Y) = 0$.

{% pf %}
Note that $(-)^+$ preserves and reflects exactness and zero-objects.

$$\begin{equation}
\mathrm{Ext}^1(X, Y^+) = H^1((P(X), Y^+)) ≃ (H^1(P(X) ⊗ Y))^+ = \mathrm{Tor}_1(X, Y)^+.
\end{equation}$$
{% endpf %}

{% endlem %}

{% ex %}
$(𝐅𝐥𝐚𝐭 , \mathcal{A})$ and $(\mathcal{A}, 𝐅𝐥𝐚𝐭 )$ are tor-torsion theories. Hence $(𝐅𝐥𝐚𝐭 , 𝐅𝐥𝐚𝐭 ^⟂ )$ is a cotorsion theory. $𝐅𝐥𝐚𝐭 ^⟂$ is known as *Enoch's cotorsion module*.

$$\begin{equation}
\mathcal{A}^+ ⊆ \text{Pure Injective} ⊆ 𝐅𝐥𝐚𝐭 ^⟂.
\end{equation}$$

{% endex %}

{% ex %}
(Torsion-free module). Recall that

$$\begin{equation}
0 → \mathrm{Tor}_1(X, R/(r)) → X ⊗ (r) → X → X ⊗ R/(r) → 0.
\end{equation}$$

If $R$ has no zero-divisor, then $\mathrm{Tor}_1(X, R/(r)) = \{xr = 0 ∣ x ∈ X\}$ is a subgroup. If $R$ is commutative domain with factional field $K$, then

$$\begin{equation}
\mathrm{Tor}_1(X,K/R) = \varinjlim_{r ∈ R ∖ \{0\}} \! \!\! ^{fil} \ \ \mathrm{Tor}(X,R/(r)) = \text{torsion subgrp of } \ X.
\end{equation}$$

A torsion-free tor-torsion theory (for general rings) is cogenerated by cyclic modules, i.e.,

$$\begin{equation}
𝐓𝐅 = {}^⊺ 𝐂𝐲𝐜𝐥𝐢𝐜 = {}^⟂ \{(R/(r))^+ : r ∈ R\}.
\end{equation}$$

{% endex %}


