---
title: $\dim ğ«ğğ©(ğ¯) - \dim \ [M] = \dim \mathrm{Ext}^1(M,M)$
author: Chencheng Zhang
layout: post
category: proof
---

## è¯æ˜

{% lem %}
(å…³é”®å…¬å¼, [è¯æ˜](Key_Lemma_Gabriel)). ä»¥ä¸‹å…³é”®å…¬å¼è”ç³»äº† Krull ç»´åº¦ä¸çº¿æ€§ç©ºé—´çš„ç»´åº¦.

$$
\dim ğ«ğğ©(ğ¯) - \dim \ [M] = \dim \mathrm{Ext}^1(M,M) = \dim \mathrm{End}(M) - q(ğ¯).
$$

{% endlem %}

{% pf %}
å¯¹è½¨é“çš„ç»´åº¦å…¬å¼

$$
\dim G = \dim \ [M] + \dim \mathrm{Stab}_{M}
$$

åšä¸€äº›è°ƒæ•´:

1. $\mathrm{Stab}_{M} = \mathrm{Aut}(M) âŠ† \mathrm{End}(M)$ æ˜¯ç¨ å¯†å¼€é›†, æ•…ç»´åº¦ç›¸åŒ;
2. Euler å‹

    $$
    q(ğ¯) = âˆ‘ _{i âˆˆ  Q_0} ğ¯_i^2 - âˆ‘ _{Î±  âˆˆ  Q_1} ğ¯_{s(Î± )}â‹…  ğ¯_{t(Î± )} = \dim G - \dim ğ«ğğ©(ğ¯);
    $$

3. é—ä¼ ä»£æ•°çš„ Euler å…¬å¼

   $$
   q(ğ¯) = \dim \mathrm{End}(M) - \dim \mathrm{Ext}^1(M,M)
   $$

å°†ä»¥ä¸Šå¸¦å…¥ Krull ç»´åº¦å…¬å¼, å¾—å…³é”®å…¬å¼.

$$
\dim ğ«ğğ©(ğ¯) - \dim \ [M] = \dim \mathrm{Ext}^1(M,M) = \dim \mathrm{End}(M) - q(ğ¯).
$$

{% endpf %}
